backend/Refinement.v
@@ -1,0 +1,423 @@
+Require Import Auto.
+Require Import Coq.Relations.Relation_Definitions.
+
+Class Refinable (A : Type) : Type :=
+  {
+    is_refinement : relation A ;
+    is_transitive : transitive A is_refinement;
+    is_right_reflexive : forall a1 a2, is_refinement a1 a2 -> is_refinement a2 a2
+  }.
+
+Infix "⊑" := is_refinement (at level 70).
+
+Arguments is_refinement : simpl never.
+
+#[export, refine] Instance refinableFun {A B} `{Refinable A} `{Refinable B} : Refinable (A -> B) :=
+  {
+    is_refinement f g := forall a1 a2, a1 ⊑ a2 -> f a1 ⊑ g a2 /\ f a1 ⊑ f a2 /\ g a1 ⊑ g a2 ;
+  }.
+Proof.
+  - intros f g h Hmono1 Hmono2 a1 a2 Hprec; split.
+    edestruct Hmono1; eauto.
+    eapply is_transitive; [ apply H1 | apply Hmono2]. eapply is_right_reflexive in Hprec; eauto.
+    split. edestruct Hmono1; clear_ctx; eauto.
+    edestruct Hmono2; clear_ctx; eauto.
+  - intros f g Hfg a a' Hprec. repeat split; edestruct Hfg; eauto; destruct H2; eauto.
+Defined.
+
+Definition sp_fun {A B} `{Refinable A} `{Refinable B} (f : A -> B): (forall a1 a2, a1 ⊑ a2 -> f a1 ⊑ f a2) -> f ⊑ f.
+Proof.
+  intros; repeat split; eauto.
+Qed.
+
+Class Complete (A : Type) `{Refinable A} :=
+  {
+    is_complete : A -> Prop ;
+    is_complete_spec : forall a, is_complete a -> a ⊑ a ;
+  }.
+
+Arguments is_complete : simpl never.
+
+#[export, refine] Instance completeFun {A B} `{Complete A} `{Complete B} : Complete (A -> B) :=
+  {
+    is_complete f := f ⊑ f /\ forall a, is_complete a -> is_complete (f a) ;
+    is_complete_spec := _;
+  }.
+Proof.
+  cbn. intros f [Hf Hcompl] a1 a2 ?; eauto.
+Defined.
+
+Lemma is_complete_const_fun : forall {A B} `{Complete A} `{Complete B} (b : B), is_complete b -> is_complete (fun _ : A => b).
+Proof.  simpl; intros. split.
+  - unfold is_refinement; cbn. eapply is_complete_spec in H3; eauto.
+  - eauto.
+Qed.
+
+#[export] Hint Resolve is_complete_const_fun : typeclass_instances.
+
+Class Ground (A : Type) `{Refinable A} `{Complete A} : Type :=
+  {
+    is_complete_minimal : forall a, is_complete a -> forall a', a' ⊑ a -> a' = a
+  }.
+
+
+Tactic Notation "unfold_complete" "in" hyp(H) := unfold is_complete in H; cbn in H.
+Tactic Notation "unfold_complete" := unfold is_complete; cbn.
+Tactic Notation "unfold_refinement" := unfold is_refinement; cbn.
+Tactic Notation "unfold_refinement" "in" hyp(H) := unfold is_refinement in H; cbn in H.
+  
+From Coq Require Import FunctionalExtensionality.
+
+Section Monotonicity.
+  Context {A} `{HAC : Complete A}.
+
+  Class Monotonizable (P : A -> Prop) :=
+    {
+      monotone : A -> Prop;
+      antitone : A -> Prop;
+      is_monotone : forall a1 a2, a1 ⊑ a2 -> monotone a1 -> monotone a2;
+      is_antitone : forall a1 a2, a1 ⊑ a2 -> antitone a2 -> antitone a1;
+      complete_monotone_is_equivalent : forall (a : A), is_complete a -> monotone a <-> P a;
+      complete_antitone_is_equivalent : forall (a : A), is_complete a -> antitone a <-> P a
+    }.
+
+  Definition monotonize (P : A -> Prop) `{Monotonizable P} : A -> Prop := monotone.
+  Definition antitonize (P : A -> Prop) `{Monotonizable P} : A -> Prop := antitone.
+
+  Corollary incompleteness_tolerance : forall (P : A -> Prop) {HP: Monotonizable P} (a1 a2 : A),
+    is_complete a1 -> a1 ⊑ a2 -> P a1 -> monotone a2.
+  Proof.
+    intros P HP a1 a2 Hac Hprec HP1.
+    eapply HP.(is_monotone); try eapply Hprec; eauto.
+    apply HP.(complete_monotone_is_equivalent); eauto.
+  Qed.
+
+  #[export] Program Instance monotonizable_const (P : Prop) : Monotonizable (fun a => P) := {
+      monotone := fun _ => P ;
+      antitone := fun _ => P ;
+      is_monotone := ltac:(eauto) ;
+      is_antitone := ltac:(eauto) ;
+      complete_monotone_is_equivalent := ltac:(now eauto) ;
+      complete_antitone_is_equivalent := ltac:(now eauto)
+    }.
+
+  #[export] Program Instance monotonizable_eq {B} `{HB : Ground B}
+    (g h : A -> B) (Hcg : is_complete g) (Hch : is_complete h)
+    : Monotonizable (fun a => g a = h a) | 2
+    := {
+      monotone := fun a => exists b, b ⊑ g a /\ b ⊑ h a ;
+      antitone := fun a => is_complete (g a) /\ g a = h a ; 
+      is_monotone := _ ;
+      is_antitone := _ ;
+      complete_monotone_is_equivalent := _ ;
+      complete_antitone_is_equivalent := _
+    }.
+  Next Obligation.
+    intros ? ? ? ? ? g h ? ? a1 a2 Hprec [b [? ?]].
+    exists b. split.
+    - apply is_transitive with (g a1) ; auto. eapply is_complete_spec in Hcg; edestruct Hcg; eauto.
+    - apply is_transitive with (h a1) ; auto. eapply is_complete_spec in Hch; edestruct Hch; eauto.
+  Qed.
+  Next Obligation.
+    intros ? ? ? ? ? g h ? ? a1 a2 Hprec [? ?].
+    erewrite (is_complete_minimal _ H3 (g a1)).
+    - split; eauto. rewrite H4 in H3.
+      erewrite (is_complete_minimal _ H3 (h a1)); eauto.
+      unfold_complete in Hch; destruct Hch as [Hhmono _].
+      apply Hhmono; eauto.
+    - unfold_complete in Hcg; destruct Hcg as [Hgmono _].
+      apply Hgmono; eauto.
+  Qed.
+  Next Obligation.
+    intros B ? ? ? ? g h Hcg Hch a Hca. split.
+    - intros [b [Hb1 Hb2]]. destruct Hcg, Hch.
+      eapply is_complete_minimal in Hb1; eauto.
+      eapply is_complete_minimal in Hb2; eauto; subst.
+      assumption.
+    - intros ->. destruct Hch. eapply is_complete_spec in Hca.
+      edestruct H3; eauto.
+  Qed.
+  Next Obligation.
+    intros B ? ? ? ? g h Hcg Hch a Hca. split.
+    - intros []; eauto.
+    - intros ->; split; eauto. unfold_complete in Hch.
+      destruct Hch as [_ Hch]; apply Hch; eauto.
+  Qed.
+
+#[export] Program Instance monotonizable_eq_2 {B} `{HB : Ground B}
+    (g : A -> B) (Hcg : is_complete g) (b : B) : Monotonizable (fun a => g a = b) | 1 := {
+      monotone := fun a => b ⊑ g a ;
+      antitone := fun a => is_complete (g a) /\ g a = b ;
+      is_monotone := _ ;
+      is_antitone := _ ;
+      complete_monotone_is_equivalent := _ ;
+      complete_antitone_is_equivalent := _
+    }.
+  Next Obligation.
+    intros ? ? ? ? ? g [Hcg ?] b a1 a2 Hprec ?.
+    apply is_transitive with (g a1); try apply Hcg; eauto.
+  Qed.
+  Next Obligation.
+  intros ? ? ? ? ? g [Hcg ?] b a1 a2 Hprec [? ?].
+  unfold_refinement in Hcg. edestruct Hcg as [Hmono ?]; eauto. apply is_complete_minimal in Hmono; eauto.
+  rewrite Hmono; eauto.
+  Qed.
+  Next Obligation.
+    intros B ? ? ? ? g [? ?] ? a Hca. split; [intros Hbg | intros <-].
+    - eapply is_complete_minimal in Hbg; eauto.
+    - apply is_complete_spec; eauto.
+  Qed.
+  Next Obligation.
+    intros B ? ? ? ? g [? ?] ? a Hca. split; [intros [? Hbg] | intros <-]; eauto.
+  Qed.
+
+  (* #[export] Program Instance monotonizable_eq_3 {B} `{HB : Ground B}
+    (g : A -> B) (Hcg : is_complete g) (b : B) : Monotonizable (fun a => b = g a) | 1 := {
+      monotone := fun a => b ⊑ g a ;
+      antitone := fun a => is_complete b /\ g a ⊑ b ;
+      is_monotone := _ ;
+      is_antitone := _ ;
+      complete_monotone_is_equivalent := _ ;
+      complete_antitone_is_equivalent := _
+    }.
+  Next Obligation.
+    intros ? ? ? ? ? g [Hcg ?] b a1 a2 Hprec ?.
+    apply is_transitive with (g a1); try apply Hcg; eauto.
+  Qed.
+  Next Obligation.
+  intros ? ? ? ? ? g [Hcg ?] b a1 a2 Hprec [? ?]; split; eauto.
+  apply is_transitive with (g a2); try apply Hcg; eauto.
+  Qed.
+  Next Obligation.
+    intros B ? ? ? ? g [? ?] ? a Hca. split; [intros Hbg | intros ->].
+    - eapply is_complete_minimal in Hbg; eauto.
+    - apply is_complete_spec; eauto.
+  Qed.
+  Next Obligation.
+    intros B ? ? ? ? g [? ?] ? a Hca. split; [intros [? Hbg] | intros ->].
+    - eapply is_complete_minimal in Hbg; eauto.
+    - split; eauto; apply is_complete_spec; eauto.
+  Qed. *)
+
+  #[export] Program Instance monotonizable_eq_fun {B C} `{HB : Refinable B} `{HC : Refinable C}
+    (g h : A -> B -> C) {Hmono : Monotonizable (fun a => forall b, g a b = h a b)} : Monotonizable (fun a => g a = h a) := {
+      monotone := Hmono.(monotone) ;
+      antitone := Hmono.(antitone) ;
+      is_monotone := _ ;
+      is_antitone := _ ;
+      complete_monotone_is_equivalent := _ ;
+      complete_antitone_is_equivalent := _
+    }.
+  Next Obligation.
+    intros B C HB HC g h Hmono a1 a2 Hprec Hmono1.
+    eapply is_monotone; eauto.
+  Qed.
+  Next Obligation.
+    intros B C HB HC g h Hmono a1 a2 Hprec Hmono1.
+    eapply is_antitone; eauto.
+  Qed.
+  Next Obligation with eauto.
+    intros B C HB HC g h Hmono a Hac; simpl; split; intros Hp.
+    - apply functional_extensionality; intros b.
+      eapply Hmono.(complete_monotone_is_equivalent)...
+    - eapply complete_monotone_is_equivalent...
+      intros b. rewrite Hp...
+  Qed.
+  Next Obligation with eauto.
+    intros B C HB HC g h Hmono a Hac; simpl; split; intros Hp.
+    - apply functional_extensionality; intros b.
+      eapply Hmono.(complete_antitone_is_equivalent)...
+    - eapply complete_antitone_is_equivalent...
+      intros b; rewrite Hp...
+  Qed.
+
+  #[export] Program Instance monotonizable_forall {B} {P : B -> A -> Prop} `{HPB : forall b, Monotonizable (P b)} : Monotonizable (fun a => forall b, P b a) :=
+    {
+      monotone := fun a => forall b, (HPB b).(monotone) a ;
+      antitone := fun a => forall b, (HPB b).(antitone) a ;
+      is_monotone := _ ;
+      is_antitone := _ ;
+      complete_monotone_is_equivalent := _ ;
+      complete_antitone_is_equivalent := _
+    }.
+  Next Obligation.
+    intros B P HPB a1 a2 Hprec Hmono; simpl; intros b.
+    eapply is_monotone.
+    - apply Hprec.
+    - eauto.
+  Qed.
+  Next Obligation.
+    intros B P HPB a1 a2 Hprec Hmono; simpl; intros b.
+    eapply is_antitone.
+    - apply Hprec.
+    - apply Hmono.
+  Qed.
+  Next Obligation with eauto.
+    intros B P HPB a Hac; simpl; split; intros HP b; eapply (HPB b).(complete_monotone_is_equivalent)...
+  Qed.
+  Next Obligation with eauto.
+    intros B P HPB a Hac; simpl; split; intros HP b; eapply (HPB b).(complete_antitone_is_equivalent)...
+  Qed.
+
+  #[export] Program Instance monotonizable_exists {B} `{HB: Refinable B} {P : B -> A -> Prop} `{HPB : forall b, Monotonizable (P b)} : Monotonizable (fun a => exists b, P b a) :=
+    {
+      monotone := fun a => exists b, (HPB b).(monotone) a ;
+      antitone := fun a => exists b, (HPB b).(antitone) a ;
+      is_monotone := _ ;
+      is_antitone := _ ;
+      complete_monotone_is_equivalent := _ ;
+      complete_antitone_is_equivalent := _
+    }.
+  Next Obligation.
+    intros B HB P HPB a1 a2 Hprec [b HP]; simpl.
+    exists b; eapply is_monotone; try apply Hprec; eauto.
+  Qed.
+  Next Obligation.
+    intros B HB P HPB a1 a2 Hprec [b HP]; simpl.
+    exists b; eapply is_antitone; try apply Hprec; eauto.
+  Qed.
+  Next Obligation with eauto.
+    intros B HB P HPB a Hac; simpl; split; intros [b HP]; exists b;
+      eapply (HPB b).(complete_monotone_is_equivalent)...
+  Qed.
+  Next Obligation with eauto.
+    intros B HB P HPB a Hac; simpl; split; intros [b HP]; exists b;
+      eapply (HPB b).(complete_antitone_is_equivalent)...
+  Qed.
+
+  #[export] Program Instance monotonizable_conj (P Q : A -> Prop) {HP : Monotonizable P} {HQ : Monotonizable Q} : Monotonizable (fun a => P a /\ Q a) :=
+    {
+      monotone := fun a => (HP.(monotone) a) /\ (HQ.(monotone) a) ;
+      antitone := fun a => (HP.(antitone) a) /\ (HQ.(antitone) a) ;
+      is_monotone := _ ;
+      is_antitone := _ ;
+      complete_monotone_is_equivalent := _ ;
+      complete_antitone_is_equivalent := _
+    }.
+  Next Obligation.
+    intros P Q HP HQ a1 a2 Hprec [HP1 HQ1]; simpl; split.
+    - eapply is_monotone; try apply Hprec; eauto.
+    - eapply is_monotone; try apply Hprec; eauto.
+  Qed.
+  Next Obligation.
+    intros P Q HP HQ a1 a2 Hprec [HP1 HQ1]; simpl; split.
+    - eapply is_antitone; try apply Hprec; eauto.
+    - eapply is_antitone; try apply Hprec; eauto.
+  Qed.
+  Next Obligation with eauto.
+    intros P Q HP HQ a Hac; simpl; split; intros [HP1 HQ1]; split; try eapply complete_monotone_is_equivalent...
+  Qed.
+  Next Obligation with eauto.
+    intros P Q HP HQ a Hac; simpl; split; intros [HP1 HQ1]; split; try eapply complete_antitone_is_equivalent...
+  Qed.
+
+  #[export] Program Instance monotonizable_disj (P Q : A -> Prop) {HP : Monotonizable P} {HQ : Monotonizable Q} : Monotonizable (fun a => P a \/ Q a) :=
+    {
+      monotone := fun a => (HP.(monotone) a) \/ (HQ.(monotone) a) ;
+      antitone := fun a => (HP.(antitone) a) \/ (HQ.(antitone) a) ;
+      is_monotone := _ ;
+      is_antitone := _ ;
+      complete_monotone_is_equivalent := _ ;
+      complete_antitone_is_equivalent := _
+    }.
+  Next Obligation.
+    intros P Q HP HQ a1 a2 Hprec [HP1 | HQ1]; simpl.
+    - left; eapply is_monotone; try apply Hprec; eauto.
+    - right; eapply is_monotone; try apply Hprec; eauto.
+  Qed.
+  Next Obligation.
+    intros P Q HP HQ a1 a2 Hprec [HP1 | HQ1]; simpl.
+    - left; eapply is_antitone; try apply Hprec; eauto.
+    - right; eapply is_antitone; try apply Hprec; eauto.
+  Qed.
+  Next Obligation with eauto.
+    intros P Q HP HQ a Hac; simpl; split; intros [HP1 | HQ1];
+      try (now left; apply complete_monotone_is_equivalent; eauto);
+      try (now right; apply complete_monotone_is_equivalent; eauto).
+  Qed.
+  Next Obligation with eauto.
+    intros P Q HP HQ a Hac; simpl; split; intros [HP1 | HQ1];
+      try (now left; apply complete_antitone_is_equivalent; eauto);
+      try (now right; apply complete_antitone_is_equivalent; eauto).
+  Qed.
+
+  #[export] Program Instance monotonizable_arrow {P Q : A -> Prop} {HP : Monotonizable P} {HQ : Monotonizable Q} : Monotonizable (fun a => P a -> Q a) :=
+    {
+      monotone := fun a => HP.(antitone) a -> HQ.(monotone) a ;
+      antitone := fun a => HP.(monotone) a -> HQ.(antitone) a ;
+      is_monotone := _ ;
+      is_antitone := _ ;
+      complete_monotone_is_equivalent := _ ;
+      complete_antitone_is_equivalent := _
+    }.
+  Next Obligation.
+    simpl; intros P Q HP HQ a1 a2 Hprec ? Hanti.
+    eapply HQ.(is_monotone).
+    - apply Hprec.
+    - apply H0. eapply HP.(is_antitone); eauto.
+  Qed.
+  Next Obligation.
+    simpl; intros P Q HP HQ a1 a2 Hprec ? Hanti.
+    eapply HQ.(is_antitone).
+    - apply Hprec.
+    - apply H0. eapply HP.(is_monotone); try apply Hprec; eauto.
+  Qed.
+  Next Obligation with eauto.
+    simpl; intros P Q HP HQ a Ha; split; intros ?.
+    - intros H1. eapply HQ.(complete_monotone_is_equivalent); eauto.
+      apply H0. eapply HP.(complete_antitone_is_equivalent); eauto.
+    - intros H1. eapply HQ.(complete_monotone_is_equivalent); eauto.
+      apply H0. eapply HP.(complete_antitone_is_equivalent); eauto.
+  Qed.
+  Next Obligation with eauto.
+    simpl; intros P Q HP HQ a Ha; split; intros ?.
+    - intros H1. eapply HQ.(complete_antitone_is_equivalent); eauto.
+      apply H0. eapply HP.(complete_monotone_is_equivalent); eauto.
+    - intros H1. eapply HQ.(complete_antitone_is_equivalent); eauto.
+      apply H0. eapply HP.(complete_monotone_is_equivalent); eauto.
+  Qed.
+
+ #[export] Program Instance monotonizable_refinement {B} `{Ground B}
+   (g : A -> B) (Hcg : is_complete g) (b : B) (Hb : is_complete b) : Monotonizable (fun a => g a ⊑ b) := {
+      monotone := fun a => b ⊑ g a ;
+      antitone := fun a => g a ⊑ b ;
+      is_monotone := _ ;
+      is_antitone := _ ;
+      complete_monotone_is_equivalent := _ ;
+      complete_antitone_is_equivalent := _
+    }.
+  Next Obligation.
+    intros ? ? ? ? ? g ? b ? a1 a2 Hprec ?.
+    apply is_transitive with (g a1); eauto.
+    apply Hcg; eauto.
+  Qed.
+  Next Obligation.
+    intros ? ? ? ? ? g ? b ? a1 a2 Hprec ?.
+    apply is_transitive with (g a2); eauto.
+    apply Hcg; eauto.
+  Qed.
+  Next Obligation.
+    intros B ? ? ? ? g ? ? ? a Hca.
+    split; intros Hbg; pose proof (Hbg' := Hbg); eapply is_complete_minimal in Hbg; eauto; try rewrite Hbg.
+    - eapply is_right_reflexive; eauto.
+    - apply Hcg; eauto.
+    - eapply is_right_reflexive; eauto.
+  Qed.
+  Next Obligation.
+    intros B ? ? ? ? g ? ? ? a Hca; split; eauto.
+  Qed.
+
+End Monotonicity.
+
+
+#[export] Hint Extern 0 (Complete _) => eassumption : typeclass_instances.
+
+Lemma fun_is_complete_if_complete_dom : forall {A B} `{Complete A} `{Complete B},
+    forall a, is_complete a -> is_complete (fun f : A -> B => f a).
+Proof.
+  simpl; intros; split.
+  - unfold is_refinement; cbn. intros. edestruct H4; eauto. eapply is_complete_spec in H3; eauto.
+  - intros. destruct H4. eauto.
+Qed.
+
+#[export] Hint Resolve fun_is_complete_if_complete_dom : typeclass_instances.
