backend/RefinementInstances.v
@@ -1,0 +1,492 @@
+Require Export Refinement.
+Require Import FunInd.
+Require Import Coqlib Maps Errors Integers Floats Lattice Kildall.
+Require Import AST Linking.
+Require Import Values Memory Globalenvs Events Smallstep.
+Require Import Registers Op RTL RTL_Incomplete.
+Require Import ValueDomain ValueAnalysis NeedDomain NeedOp.
+
+(* Destructs conjunctions, disjunctions, etc. *)
+Ltac destruct_ctx := 
+  repeat (match goal with
+  | [H : _ \/ _ |- _ ] => 
+    let Hl := fresh H in 
+    let Hr := fresh H in
+    destruct H as [Hl | Hr]
+  | [H : _ /\ _ |- _ ] => 
+    let Hl := fresh H in 
+    let Hr := fresh H in
+    destruct H as [Hl Hr]
+  | [H : _ <-> _ |- _ ] => 
+    let Hl := fresh H in 
+    let Hr := fresh H in
+    destruct H as [Hl Hr]
+  | [H : exists (x : _), _ |- _ ] =>
+    let x := fresh x in
+    destruct H as [x H]
+  | [H : ?P , H2 : ?P |- _ ] => clear H2
+  end
+  ).
+
+
+(* Makes refinable instances where the refinement relation is equality. *)
+Definition mkEqRefinable (A : Type) : Refinable A :=
+ {|
+  is_refinement (x y : A) := x = y ;
+  is_transitive := ltac:(unfold Relation_Definitions.transitive; try induction x; eauto; intros; subst; eauto);
+  is_right_reflexive := ltac:(simpl; eauto) ;
+  |}.
+
+(* Makes complete instances where the complete predicate is always true. 
+  The premise is just to reuse the definition for other types with eq refinement.
+*)
+Program Definition mkCompleteTrue (A : Type) (refEqA := mkEqRefinable A) : Complete A :=
+  {|
+    is_complete _:= True ;
+    is_complete_spec := _
+  |}.
+Next Obligation. reflexivity. Qed.
+
+Program Definition mkGroundTrue (A : Type) (refEqA := mkEqRefinable A) (compA := mkCompleteTrue A) : Ground A :=
+  {|
+    is_complete_minimal := _
+  |}.
+
+#[export, refine] Instance refinableRes {A} `{Refinable A} : Refinable (res A) := 
+{
+  is_refinement r1 r2 := match r1, r2 with 
+  | OK x1, OK x2 => x1 ⊑ x2
+  (* Just to get ground *)
+  | Error e1, Error e2 => e1 = e2
+  | _, _ => False
+  end
+}.
+Proof.
+  - unfold Relation_Definitions.transitive; intros [] [] [] ? ?; eauto; try contradiction.
+    * eapply is_transitive; eauto.
+    * subst; eauto.
+  - intros [] []; eauto; try eapply is_right_reflexive; eauto; try contradiction.
+Defined.
+
+#[export, refine] Instance completeRes {A} `{Complete A} : Complete (res A) := 
+  {
+    is_complete := fun r => match r with
+    | OK x => is_complete x
+    | Error _ => True
+    end
+  }.
+Proof.
+  intros []; eauto; intros; simpl; eauto; unfold is_refinement; cbn; try apply is_complete_spec; eauto.
+Defined.
+
+#[export] Instance groundRes {A} `{Ground A} : Ground (res A).
+Proof. constructor; intros [] ? []; simpl; try contradiction; intros.
+      - f_equal. eapply is_complete_minimal; eauto.
+      - unfold is_refinement in H4; cbn in H4; subst; eauto.
+Defined. 
+
+#[export, refine] Instance refinableOption {A} `{Refinable A} : Refinable (option A) := 
+{
+  is_refinement o1 o2 := match o1, o2 with 
+  | Some x1, Some x2 => x1 ⊑ x2
+  | None, None => True
+  | _, _ => False
+  end
+}.
+Proof.
+  - unfold Relation_Definitions.transitive; intros [] [] [] ? ?; eauto; try contradiction.
+    eapply is_transitive; eauto.
+  - intros [] []; eauto; try eapply is_right_reflexive; eauto; try contradiction.
+Defined.
+
+#[export, refine] Instance completeOption {A} `{Complete A} : Complete (option A) := 
+  {
+    is_complete := fun o => match o with
+    | Some x => is_complete x
+    | None => True
+    end
+  }.
+Proof.
+  intros []; eauto; intros; simpl; eauto. unfold is_refinement; cbn; apply is_complete_spec; eauto.
+Defined.
+
+#[export] Instance groundOption {A} `{Ground A} : Ground (option A).
+Proof. constructor; intros [] ? []; simpl; try contradiction; intros; eauto.
+      f_equal. eapply is_complete_minimal; eauto.
+Defined. 
+
+#[export, refine] Instance refinableList {A} `{Refinable A} : Refinable (list A) := 
+{
+  is_refinement l1 l2 := let fix aux l1 l2 :=
+   match l1, l2 with
+    | nil, nil => True
+    | x :: xs, y :: ys => x ⊑ y /\ aux xs ys
+    | _, _ => False
+    end in aux l1 l2
+}.
+Proof.
+  - unfold Relation_Definitions.transitive. induction x; intros; destruct y; eauto; try contradiction.
+    destruct z; eauto; try contradiction. destruct H0; destruct H1; split; try eapply is_transitive; eauto.
+    eapply IHx; eauto.
+  - intros l1; induction l1; intros []; eauto; try contradiction; simpl. intros []; split; try eapply is_right_reflexive; eauto. 
+  apply IHl1; eauto.
+Defined.
+
+#[export, refine] Instance completeList {A} `{Complete A} : Complete (list A) := 
+  {
+    is_complete l := let fix aux l := 
+    match l with 
+    | nil => True 
+    | x :: xs => is_complete x /\ aux xs
+    end in aux l
+  }.
+Proof.
+  intros l; induction l; eauto. simpl; intros []; constructor; try eapply is_complete_spec; eauto.
+  apply IHl; eauto.
+Defined.
+
+#[export] Instance groundList {A} `{Ground A} : Ground (list A).
+Proof. constructor; intros l; induction l; intros [] []; try contradiction; eauto.
+  intros []. f_equal. eapply is_complete_minimal; eauto.
+  apply IHl; eauto.
+Defined.
+  
+#[export, refine] Instance refinableSum {A B} `{Refinable A} `{Refinable B} : Refinable (A + B) := 
+{
+  is_refinement s1 s2 := match s1, s2 with 
+  | inl x1, inl x2 => x1 ⊑ x2
+  | inr y1, inr y2 => y1 ⊑ y2
+  | _, _ => False
+  end
+}.
+Proof.
+  - unfold Relation_Definitions.transitive; intros [] [] [] ? ?; eauto; try contradiction; eapply is_transitive; eauto.
+  - intros [] []; eauto; try eapply is_right_reflexive; eauto; try contradiction.
+Defined.
+
+#[export, refine] Instance completeSum {A B} `{Complete A} `{Complete B} : Complete (A + B) := 
+  {
+    is_complete := fun s => match s with
+    | inl x => is_complete x
+    | inr y => is_complete y
+    end
+  }.
+Proof.
+  intros []; eauto; intros; simpl; eauto; unfold_refinement; eapply is_complete_spec; eauto.
+Defined.
+
+#[export] Instance groundSum {A B} `{Ground A} `{Ground B} : Ground (A + B).
+Proof. constructor; intros [] ? []; simpl; try contradiction; intros; eauto; f_equal; eapply is_complete_minimal; eauto.
+Defined.
+
+#[export, refine] Instance refinableProd {A B} `{Refinable A} `{Refinable B} : Refinable (A * B) := 
+{
+  is_refinement p1 p2 := let (x1, y1) := p1 in let (x2, y2) := p2 in x1 ⊑ x2 /\ y1 ⊑ y2
+}.
+Proof.
+  - unfold Relation_Definitions.transitive; intros [] [] [] [] []; split; try eapply is_transitive; eauto.
+  - intros [] [] []; split; try eapply is_right_reflexive; eauto.
+Defined.
+
+#[export, refine] Instance completeProd {A B} `{Complete A} `{Complete B} : Complete (A * B) := 
+  {
+    is_complete := fun p => let (x, y) := p in is_complete x /\ is_complete y
+  }.
+Proof.
+  intros [] []; constructor; try eapply is_complete_spec; eauto.
+Defined.
+
+#[export] Instance groundProd {A B} `{Ground A} `{Ground B} : Ground (A * B).
+Proof. constructor; intros [] [] [] []; f_equal; eapply is_complete_minimal; eauto. 
+Defined. 
+
+Arguments monotone {A} {H} {HAC} P {Monotonizable}.
+#[export, refine] Instance monoForall2 {A B C} `{Complete C} (l1 : list A) (l2 : list B) (f : C -> A -> B -> Prop) {Hf : forall a b, Monotonizable (fun c => f c a b)} : Monotonizable (fun c => list_forall2 (f c) l1 l2) := 
+{
+  monotone := fun c => list_forall2 (fun a b => (Hf a b).(monotone (fun c => f c a b)) c) l1 l2;
+  antitone := fun c => list_forall2 (fun a b => (Hf a b).(antitone) c) l1 l2;
+}.
+Proof.
+  - intros ? ? ?; induction 1; constructor; eauto. eapply is_monotone; eauto.
+  - intros ? ? ?; induction 1; constructor; eauto. eapply is_antitone; eauto.
+  - intros c ?; split; induction 1; econstructor; eauto.
+    * eapply (Hf a1 b1).(complete_monotone_is_equivalent); eauto.
+    * eapply (Hf a1 b1).(complete_monotone_is_equivalent); eauto.
+  - intros c ?; split; induction 1; econstructor; eauto; eapply (Hf a1 b1).(complete_antitone_is_equivalent); eauto.
+Defined.
+  
+(* node and reg are positive *)
+#[export] Instance : Refinable reg := mkEqRefinable reg.
+#[export] Instance : Complete reg := mkCompleteTrue reg. 
+#[export] Instance : Ground reg := mkGroundTrue reg.
+
+#[export] Instance : Refinable operation := mkEqRefinable operation.
+#[export] Instance : Complete operation := mkCompleteTrue operation.
+
+#[export] Instance : Refinable memory_chunk := mkEqRefinable memory_chunk.
+#[export] Instance : Complete memory_chunk := mkCompleteTrue memory_chunk.
+
+#[export] Instance : Refinable addressing := mkEqRefinable addressing. 
+#[export] Instance : Complete addressing := mkCompleteTrue addressing.
+
+(* Signature is actually a record *)
+#[export] Instance : Refinable signature := mkEqRefinable signature.
+#[export] Instance : Complete signature := mkCompleteTrue signature.
+#[export] Instance : Ground signature := mkGroundTrue signature.
+
+(* external_function is an inductive *)
+#[export] Instance : Refinable external_function := mkEqRefinable external_function.
+#[export] Instance : Complete external_function := mkCompleteTrue external_function.
+#[export] Instance : Ground external_function := mkGroundTrue external_function.
+
+#[export] Instance : Refinable condition := mkEqRefinable condition.
+#[export] Instance : Complete condition := mkCompleteTrue condition.
+
+(* builtin_arg and res are parameterized, so one could have a more general definition *)
+#[export] Instance : Refinable (builtin_arg reg) := mkEqRefinable (builtin_arg reg).
+#[export] Instance : Complete (builtin_arg reg) := mkCompleteTrue (builtin_arg reg).
+
+#[export] Instance : Refinable (builtin_res reg) := mkEqRefinable (builtin_res reg).
+#[export] Instance : Complete (builtin_res reg) := mkCompleteTrue (builtin_res reg).
+
+#[export] Instance : Refinable ablock := mkEqRefinable ablock.
+#[export] Instance : Complete ablock := mkCompleteTrue ablock.
+
+#[export] Instance : Refinable Z := mkEqRefinable Z.
+#[export] Instance : Complete Z := mkCompleteTrue Z . 
+#[export] Instance : Ground Z := mkGroundTrue Z . 
+
+#[export] Instance : Refinable init_data := mkEqRefinable init_data.
+#[export] Instance : Complete init_data := mkCompleteTrue init_data.
+
+#[export] Instance : Refinable bool := mkEqRefinable bool.
+#[export] Instance : Complete bool := mkCompleteTrue bool.
+
+#[export] Instance : Refinable ident := mkEqRefinable ident.
+
+#[export] Instance : Refinable unit := mkEqRefinable unit.
+#[export] Instance : Complete unit := mkCompleteTrue unit.
+
+#[export] Instance : Refinable val := mkEqRefinable val.
+#[export] Instance : Complete val := mkCompleteTrue val.
+#[export] Instance : Ground val := mkGroundTrue val.
+
+#[export] Instance : Refinable mem := mkEqRefinable mem.
+#[export] Instance : Complete mem := mkCompleteTrue mem.
+#[export] Instance : Ground mem := mkGroundTrue mem.
+
+#[export] Instance : Refinable RTL.instruction := mkEqRefinable RTL.instruction.
+#[export] Instance : Complete RTL.instruction := mkCompleteTrue RTL.instruction.
+#[export] Instance : Ground RTL.instruction := mkGroundTrue RTL.instruction.
+
+#[export] Program Instance refinableInstruction : Refinable instruction :=
+  {|
+    is_refinement i1 i2 := 
+        match i1, i2 with
+        | Inop n1, Inop n2 => n1 ⊑ n2
+        | Iop op1 args1 res1 n1, Iop op2 args2 res2 n2 => op1 ⊑ op2 /\ args1 ⊑ args2 /\ res1 ⊑ res2 /\ n1 ⊑ n2
+        | Iload chunk1 addr1 args1 res1 n1, Iload chunk2 addr2 args2 res2 n2 => chunk1 ⊑ chunk2 /\ addr1 ⊑ addr2 /\ args1 ⊑ args2 /\ res1 ⊑ res2 /\ n1 ⊑ n2
+        | Istore chunk1 addr1 args1 args1' n1, Istore chunk2 addr2 args2 args2' n2 => chunk1 ⊑ chunk2 /\ addr1 ⊑ addr2 /\ args1 ⊑ args2 /\ args1' ⊑ args2' /\ n1 ⊑ n2
+        | Icall sig1 ros1 args1 res1 n1, Icall sig2 ros2 args2 res2 n2 => sig1 ⊑ sig2 /\ ros1 ⊑ ros2 /\ args1 ⊑ args2 /\ res1 ⊑ res2 /\ n1 ⊑ n2
+        | Itailcall sig1 ros1 args1, Itailcall sig2 ros2 args2 => sig1 ⊑ sig2 /\ ros1 ⊑ ros2 /\ args1 ⊑ args2
+        | Ibuiltin ef1 args1 res1 n1, Ibuiltin ef2 args2 res2 n2 => ef1 ⊑ ef2 /\ args1 ⊑ args2 /\ res1 ⊑ res2 /\ n1 ⊑ n2
+        | Icond cond1 args1 n11 n12, Icond cond2 args2 n21 n22 => cond1 ⊑ cond2 /\ args1 ⊑ args2 /\ n11 ⊑ n21 /\ n12 ⊑ n22
+        | Ijumptable r1 n1, Ijumptable r2 n2 => r1 ⊑ r2 /\ n1 ⊑ n2
+        | Ireturn mr1, Ireturn mr2 => mr1 ⊑ mr2
+        | _, Inotimplemented => True
+        | _, _ => False
+        end
+  |}.
+Admit Obligations.
+
+Inductive is_complete_instruction : instruction -> Prop :=
+| is_complete_Inop : forall n, is_complete n -> is_complete_instruction (Inop n)
+| is_complete_Iop : forall op args res n, is_complete op -> is_complete args -> is_complete res -> is_complete n -> is_complete_instruction (Iop op args res n)
+| is_complete_Iload : forall chunk addr args res n, is_complete chunk -> is_complete addr -> is_complete args -> is_complete res -> is_complete n -> is_complete_instruction (Iload chunk addr args res n)
+| is_complete_Istore : forall chunk addr args args' n, is_complete chunk -> is_complete addr -> is_complete args -> is_complete args' -> is_complete n -> is_complete_instruction (Istore chunk addr args args' n)
+| is_complete_Icall : forall sig ros args res n, is_complete sig -> is_complete ros -> is_complete args -> is_complete res -> is_complete n -> is_complete_instruction (Icall sig ros args res n)
+| is_complete_Itailcall : forall sig ros args, is_complete sig -> is_complete ros -> is_complete args -> is_complete_instruction (Itailcall sig ros args)
+| is_complete_Ibuiltin : forall ef args res n, is_complete ef -> is_complete args -> is_complete res -> is_complete n -> is_complete_instruction (Ibuiltin ef args res n)
+| is_complete_Icond : forall cond args n1 n2, is_complete cond -> is_complete args -> is_complete n1 -> is_complete n2 -> is_complete_instruction (Icond cond args n1 n2)
+| is_complete_Ijumptable : forall r n, is_complete r -> is_complete n -> is_complete_instruction (Ijumptable r n)
+| is_complete_Ireturn : forall mr, is_complete mr -> is_complete_instruction (Ireturn mr).
+
+#[export] Program Instance completeInstruction : Complete instruction := 
+{ 
+  is_complete := is_complete_instruction
+}.
+Admit Obligations.
+
+#[export] Instance groundInstruction : Ground instruction. 
+Proof. Admitted.
+
+#[export] Program Instance refinablePTree {A} `{Refinable A} : Refinable (PTree.t A) := 
+{
+  is_refinement t1 t2 := forall pc, t1 ! pc ⊑ t2 ! pc  
+}.
+Admit Obligations.
+
+#[export] Program Instance completePTree {A} `{Complete A} : Complete (PTree.t A) := 
+{
+  is_complete t := forall pc, is_complete (t ! pc)
+}.
+Admit Obligations.
+
+#[export] Program Instance groundPTree {A} `{Ground A} : Ground (PTree.t A) := 
+{
+  is_complete_minimal := _
+}.
+Admit Obligations.
+
+#[export] Instance : Refinable romem. apply refinablePTree. Defined.
+#[export] Instance : Complete romem. apply completePTree. Defined.
+Lemma romem_complete : forall r : romem, is_complete r. 
+Proof. intros; unfold_complete; intros; unfold_complete; destruct (_ ! _); try unfold_complete; eauto. Qed.
+Lemma romem_sp : forall r : romem, r ⊑ r. 
+Proof. intros; unfold_refinement; intros; unfold_refinement; destruct (_ ! _); try unfold_refinement; eauto. Qed.
+
+
+#[export] Instance : Refinable RTL.function := mkEqRefinable RTL.function.
+#[export] Instance : Complete RTL.function := mkCompleteTrue RTL.function.
+
+#[export, refine] Instance : Refinable function := 
+  {
+    is_refinement f1 f2 := 
+    (fn_sig f1) ⊑ (fn_sig f2) /\ (fn_params f1) ⊑ (fn_params f2) /\ (fn_stacksize f1) ⊑ (fn_stacksize f2) /\ (fn_code f1) ⊑ (fn_code f2) /\ (fn_entrypoint f1) ⊑ (fn_entrypoint f2)
+  }.
+Proof. 
+  - unfold Relation_Definitions.transitive; intros [] [] [] ? ?.
+    destruct_ctx.
+    repeat split; try eapply is_transitive; eauto.
+  - intros [] [] ?; destruct_ctx. repeat split; try eapply is_right_reflexive; eauto.
+Defined.
+
+
+#[export] Program Instance : Complete function := {
+  is_complete f := 
+  is_complete (fn_sig f) /\ is_complete (fn_params f) /\ is_complete (fn_stacksize f) /\ is_complete (fn_code f) /\ is_complete (fn_entrypoint f)
+  (* forall pc, is_complete pc -> is_complete ((fn_code f) ! pc) *)
+}.
+Admit Obligations.
+
+#[export] Instance : Ground function.
+Proof. constructor. intros [] HC [] HR. unfold_complete in HC; unfold_refinement in HR. destruct_ctx. unshelve f_equal; unshelve eapply is_complete_minimal; eauto; try typeclasses eauto.
+Defined.
+
+
+#[export] Program Instance refinableGlobvar {V} `{Refinable V} : Refinable (globvar V) := 
+{
+  is_refinement g1 g2 := (gvar_info g1) ⊑ (gvar_info g2) /\ (gvar_init g1) ⊑ (gvar_init g2) /\ (gvar_readonly g1) ⊑ (gvar_readonly g2) /\ (gvar_volatile g1) ⊑ (gvar_volatile g2)
+}.
+Admit Obligations.
+
+#[export] Program Instance completeGlobvar {V} `{Complete V} : Complete (globvar V) := 
+{
+  is_complete g := is_complete (gvar_info g) /\ is_complete (gvar_init g) /\ is_complete (gvar_readonly g) /\ is_complete (gvar_volatile g)
+}.
+Admit Obligations.
+
+Inductive is_refinement_globdef {F V} `{Refinable F} `{Refinable V} : globdef F V -> globdef F V -> Prop :=
+| is_refinement_Gfun : forall f1 f2, f1 ⊑ f2 -> is_refinement_globdef (Gfun f1) (Gfun f2)
+| is_refinement_Gvar : forall v1 v2, v1 ⊑ v2 -> is_refinement_globdef (Gvar v1) (Gvar v2).
+
+#[export] Program Instance refinableGlobdef {F V} `{Refinable F} `{Refinable V} : Refinable (globdef F V) := 
+{
+  is_refinement := is_refinement_globdef
+}.
+Admit Obligations.
+
+Inductive is_complete_globdef {F V} `{Complete F} `{Complete V} : globdef F V -> Prop :=
+| is_complete_Gfun : forall f, is_complete f -> is_complete_globdef (Gfun f)
+| is_complete_Gvar : forall v, is_complete v -> is_complete_globdef (Gvar v).
+
+#[export] Program Instance completeGlobdef {F V} `{Complete F} `{Complete V} : Complete (globdef F V) := 
+{
+  is_complete := is_complete_globdef
+}.
+Admit Obligations.
+
+
+#[export] Program Instance refinableASTFundef {F} `{Refinable F} : Refinable (AST.fundef F) := 
+{
+  is_refinement fd1 fd2 := 
+    match fd1, fd2 with
+    | External ef1, External ef2 => ef1 ⊑ ef2
+    | Internal f1, Internal f2 => f1 ⊑ f2
+    | _, _ => False
+    end
+}.
+Admit Obligations.
+
+#[export] Program Instance completeASTFundef {F} `{Complete F} : Complete (AST.fundef F) := 
+{
+  is_complete fd := 
+    match fd with
+    | External ef => is_complete ef
+    | Internal f => is_complete f
+    end
+}.
+Admit Obligations. 
+
+#[export] Instance groundASTFundef {F} `{Ground F} : Ground (AST.fundef F).
+Proof. constructor. intros [] ? [] ?; try contradiction;
+  try f_equal; eauto; eapply is_complete_minimal; eauto.
+Qed.
+
+#[export] Instance : Refinable fundef. apply refinableASTFundef. Defined.
+#[export] Instance : Complete fundef. apply completeASTFundef. Defined.
+#[export] Instance : Ground fundef. Admitted.
+
+#[export] Instance : Refinable RTL.program := mkEqRefinable RTL.program.
+#[export] Instance : Complete RTL.program := mkCompleteTrue RTL.program.
+
+#[export] Program Instance refinableASTProgram : Refinable program := 
+{
+  is_refinement p1 p2 := forall ros rs, find_function (Genv.globalenv p1) ros rs ⊑ find_function (Genv.globalenv p2) ros rs
+}.
+Admit Obligations.
+
+#[export] Program Instance completeASTProgram : Complete program := 
+{
+  is_complete p := (forall ros rs, is_complete (find_function (Genv.globalenv p) ros rs)) /\ forall b, is_complete (Genv.find_funct_ptr (Genv.globalenv p) b)
+}.
+Admit Obligations.
+
+#[export] Instance : Refinable program. apply refinableASTProgram. Defined.
+#[export] Instance : Complete program. apply completeASTProgram. Defined.
+
+#[export] Instance : Refinable code. apply refinablePTree. Defined.
+#[export] Instance : Complete code. apply completePTree. Defined.
+#[export] Instance : Ground code. apply groundPTree. Defined.
+
+#[export] Instance : Refinable code. apply refinablePTree. Defined.
+#[export] Instance : Complete code. apply completePTree. Defined.
+#[export] Instance : Ground code. apply groundPTree. Defined.
+
+
+#[export, refine] Instance : Refinable stackframe := 
+{
+  is_refinement '(Stackframe r1 f1 v1 n1 rs1) '(Stackframe r2 f2 v2 n2 rs2) := 
+  r1 ⊑ r2 /\ f1 ⊑ f2 /\ v1 ⊑ v2 /\ n1 ⊑ n2 /\ rs1 ⊑ rs2
+}.
+Proof.
+  - unfold Relation_Definitions.transitive; intros [] [] [] ? ?; destruct_ctx.
+    unfold_refinement in H7; unfold_refinement in H0; destruct_ctx. 
+    repeat split; eapply is_transitive; eauto.
+  - intros [] [] ?; destruct_ctx. unfold_refinement in H2; destruct_ctx.
+    repeat split; try eapply is_right_reflexive; eauto.
+Defined.
+
+Inductive is_refinement_state : state -> state -> Prop :=
+| is_refinement_State : forall sfr1 sfr2 f1 f2 v1 v2 n1 n2 r1 r2 m1 m2, 
+  sfr1 ⊑ sfr2 -> f1 ⊑ f2 -> v1 ⊑ v2 -> n1 ⊑ n2 -> r1 ⊑ r2 -> m1 ⊑ m2 -> is_refinement_state (State sfr1 f1 v1 n1 r1 m1) (State sfr2 f2 v2 n2 r2 m2)
+| is_refinement_Callstate : forall sfr1 sfr2 fd1 fd2 v1 v2 m1 m2,
+  sfr1 ⊑ sfr2 -> fd1 ⊑ fd2 -> v1 ⊑ v2 -> m1 ⊑ m2 -> is_refinement_state (Callstate sfr1 fd1 v1 m1) (Callstate sfr2 fd2 v2 m2)
+| is_refinement_Returnstate : forall sfr1 sfr2 v1 v2 m1 m2, 
+  sfr1 ⊑ sfr2 -> v1 ⊑ v2 -> m1 ⊑ m2 -> is_refinement_state (Returnstate sfr1 v1 m1) (Returnstate sfr2 v2 m2).
+
+#[export] Program Instance : Refinable state := 
+{
+  is_refinement := is_refinement_state
+}.
+Admit Obligations.
